Modal/modal/sound_complete/K_kripke.lean
@@ -10,11 +10,11 @@ open Modal.ProofSystems Modal.Models
 def all_frames : Kripke.Frame → Prop := fun _ => True
 
 theorem is_sound_strong (Atom : Type) :
-    Logic.is_sound_strong (K.proof_system Atom) (@Kripke.semantics Atom all_frames) :=
+    Logic.is_sound_strong (K.proof_system Atom) Kripke.semantics :=
   by admit
 
 theorem is_complete_weak (Atom : Type) :
-     Logic.is_complete_weak (K.proof_system Atom) (@Kripke.semantics Atom all_frames) :=
+     Logic.is_complete_weak (K.proof_system Atom) Kripke.semantics :=
   by admit
 -- K is not strongly complete wrt Kripke models
 
